src/Helpers/Sorting.v
@@ -1,0 +1,79 @@
+Require Import Permutation.
+Require Import Recdef.
+Require List.
+
+Import List.ListNotations.
+Open Scope list.
+
+Section Sorting.
+  Context {A:Type}.
+  Variable lt: A -> A -> bool.
+  Infix "<?" := lt (at level 20).
+
+  Fixpoint insert (x: A) (xs: list A) : list A :=
+    match xs with
+    | nil => [x]
+    | x'::xs' => if x <? x'
+                 then x::x'::xs'
+                 else x'::insert x xs'
+    end.
+
+  Hint Constructors Permutation.
+
+  Theorem inserted_permutation : forall x xs,
+      Permutation (x::xs) (insert x xs).
+  Proof.
+    induction xs; simpl; eauto.
+    destruct (x <? a); eauto.
+  Qed.
+
+  Fixpoint insert_sort (xs: list A) (acc: list A) : list A :=
+    match xs with
+      | nil => acc
+      | x::xs => insert_sort xs (insert x acc)
+    end.
+
+  Definition sort xs := insert_sort xs [].
+
+  Theorem insert_sort_permutation : forall xs acc,
+      Permutation (xs++acc) (insert_sort xs acc).
+  Proof.
+    induction xs; intros; simpl.
+    - auto.
+    - etransitivity; [ | eauto ].
+      pose proof (inserted_permutation a acc).
+      transitivity (xs ++ a :: acc).
+      apply Permutation_cons_app; auto.
+      apply Permutation_app; auto.
+  Qed.
+
+  Theorem sort_permutation : forall xs,
+      Permutation xs (sort xs).
+  Proof.
+    unfold sort.
+    intros.
+    replace xs with (xs ++ []) at 1.
+    apply insert_sort_permutation.
+    rewrite List.app_nil_r; auto.
+  Qed.
+
+End Sorting.
+
+Require Import PeanoNat.
+
+Definition sortBy {A} (key: A -> option nat) (xs: list A) : list A :=
+  sort (fun x y => Nat.leb (match key x with
+                            | Some n => S n
+                            | None => 0
+                            end)
+                           (match key y with
+                            | Some n => S n
+                            | None => 0
+                            end)) xs.
+
+Theorem sortBy_permutation : forall A key (xs: list A),
+    Permutation xs (sortBy key xs).
+Proof.
+  unfold sortBy; intros.
+  apply sort_permutation.
+Qed.
